dfny

YEAR 3/CS357 (Software Verification)/week7/q3/q3.dfy
@@ -6,56 +6,13 @@ function SumTo(a: array<int>, i: nat): int
 }
 
 method CumulativeSum(a: array<int>)
-    // needs modifies clause and postcondition
     modifies a
-    requires a != null
-    requires a.Length > 1
-    ensures forall i :: 0 <= i < a.Length ==> a[i] == SumTo(a, i)
-    
 {
-    // todo
-    var i:=0;
-    //var sum:= 0;
-    
-    while i < a.Length
+    var sum := 0;
+    for i := 0 to a.Length
         invariant 0 <= i <= a.Length
-        //invariant sum == SumTo(a, i)
-        invariant forall j :: 0 <= j < i ==> a[j] == SumTo(a, j)
+        invariant sum == SumTo(a, i)
     {
-        //sum:= SumTo(a, i);
-        a[i]:= SumTo(a, i);
-        i:= i+1;
+        sum := sum + a[i];
     }
 }
-
-/* 
-function SumTo(a: array<int>, i: nat): int
-    reads a
-    requires 0 <= i <= a.Length
-{
-    if i == 0 then 0 else SumTo(a, i - 1) + a[i - 1]
-}
-
-method CumulativeSum(a: array<int>)
-    requires a != null
-    requires a.Length >= 1
-    modifies a
-    ensures forall x | 0 <= x < a.Length :: a[x] == SumTo(a,x)
-{
-    a[0] := a[0];
-    var i := 1;
-
-    while i < a.Length
-        invariant a[0] == SumTo(a,0)
-        invariant 1 <= i <= a.Length
-
-        //ERROR : invariant might not be maintained by the loop.
-        invariant forall j :: 0 <= x < i ==> a[j] == SumTo(a,j+1)
-
-        decreases a.Length - i
-    {
-        a[i] := a[i] + a[i-1];
-        i := i + 1;
-    }
-}
- */
